work around to define  evalForExpression

fr.inria.atlanmod.coqtl.coq/.coqdeps.d
@@ -1,5 +1,5 @@
-core/utils/tArith.vo core/utils/tArith.glob core/utils/tArith.v.beautified: core/utils/tArith.v
-core/utils/tArith.vio: core/utils/tArith.v
+core/utils/tArith.vo core/utils/tArith.glob core/utils/tArith.v.beautified: core/utils/tArith.v core/utils/tNotation.vo
+core/utils/tArith.vio: core/utils/tArith.v core/utils/tNotation.vio
 core/utils/tList.vo core/utils/tList.glob core/utils/tList.v.beautified: core/utils/tList.v
 core/utils/tList.vio: core/utils/tList.v
 core/utils/tConcat.vo core/utils/tConcat.glob core/utils/tConcat.v.beautified: core/utils/tConcat.v core/utils/tList.vo
@@ -14,29 +14,49 @@ core/utils/tNotation.vo core/utils/tNotation.glob core/utils/tNotation.v.beautif
 core/utils/tNotation.vio: core/utils/tNotation.v
 core/utils/tTop.vo core/utils/tTop.glob core/utils/tTop.v.beautified: core/utils/tTop.v core/utils/tArith.vo core/utils/tList.vo core/utils/tTuple.vo core/utils/tConcat.vo core/utils/tNotation.vo core/utils/tString.vo core/utils/tPrint.vo
 core/utils/tTop.vio: core/utils/tTop.v core/utils/tArith.vio core/utils/tList.vio core/utils/tTuple.vio core/utils/tConcat.vio core/utils/tNotation.vio core/utils/tString.vio core/utils/tPrint.vio
+core/utils/CpdtTactics.vo core/utils/CpdtTactics.glob core/utils/CpdtTactics.v.beautified: core/utils/CpdtTactics.v
+core/utils/CpdtTactics.vio: core/utils/CpdtTactics.v
 core/Metamodel.vo core/Metamodel.glob core/Metamodel.v.beautified: core/Metamodel.v core/Model.vo
 core/Metamodel.vio: core/Metamodel.v core/Model.vio
 core/Model.vo core/Model.glob core/Model.v.beautified: core/Model.v
 core/Model.vio: core/Model.v
 core/Engine.vo core/Engine.glob core/Engine.v.beautified: core/Engine.v core/utils/tTop.vo core/Model.vo
 core/Engine.vio: core/Engine.v core/utils/tTop.vio core/Model.vio
-core/CoqTL.vo core/CoqTL.glob core/CoqTL.v.beautified: core/CoqTL.v core/Metamodel.vo core/Model.vo core/Engine.vo core/utils/tTop.vo
-core/CoqTL.vio: core/CoqTL.v core/Metamodel.vio core/Model.vio core/Engine.vio core/utils/tTop.vio
+core/CoqTL.vo core/CoqTL.glob core/CoqTL.v.beautified: core/CoqTL.v core/Metamodel.vo core/Model.vo core/Engine.vo core/utils/tTop.vo core/utils/tArith.vo core/utils/CpdtTactics.vo
+core/CoqTL.vio: core/CoqTL.v core/Metamodel.vio core/Model.vio core/Engine.vio core/utils/tTop.vio core/utils/tArith.vio core/utils/CpdtTactics.vio
 core/Notations.vo core/Notations.glob core/Notations.v.beautified: core/Notations.v core/CoqTL.vo
 core/Notations.vio: core/Notations.v core/CoqTL.vio
-examples/Class2Relational/ClassMetamodel.vo examples/Class2Relational/ClassMetamodel.glob examples/Class2Relational/ClassMetamodel.v.beautified: examples/Class2Relational/ClassMetamodel.v core/utils/tTop.vo core/Metamodel.vo core/Model.vo
-examples/Class2Relational/ClassMetamodel.vio: examples/Class2Relational/ClassMetamodel.v core/utils/tTop.vio core/Metamodel.vio core/Model.vio
-examples/Class2Relational/RelationalMetamodel.vo examples/Class2Relational/RelationalMetamodel.glob examples/Class2Relational/RelationalMetamodel.v.beautified: examples/Class2Relational/RelationalMetamodel.v core/utils/tTop.vo core/Metamodel.vo core/Model.vo
-examples/Class2Relational/RelationalMetamodel.vio: examples/Class2Relational/RelationalMetamodel.v core/utils/tTop.vio core/Metamodel.vio core/Model.vio
-examples/Class2Relational/Class2Relational.vo examples/Class2Relational/Class2Relational.glob examples/Class2Relational/Class2Relational.v.beautified: examples/Class2Relational/Class2Relational.v core/utils/tTop.vo core/Notations.vo core/CoqTL.vo examples/Class2Relational/ClassMetamodel.vo examples/Class2Relational/RelationalMetamodel.vo
-examples/Class2Relational/Class2Relational.vio: examples/Class2Relational/Class2Relational.v core/utils/tTop.vio core/Notations.vio core/CoqTL.vio examples/Class2Relational/ClassMetamodel.vio examples/Class2Relational/RelationalMetamodel.vio
+core/Object.vo core/Object.glob core/Object.v.beautified: core/Object.v
+core/Object.vio: core/Object.v
+examples/Class2Relational/ClassMetamodel.vo examples/Class2Relational/ClassMetamodel.glob examples/Class2Relational/ClassMetamodel.v.beautified: examples/Class2Relational/ClassMetamodel.v core/utils/tTop.vo core/Metamodel.vo core/Model.vo core/Object.vo
+examples/Class2Relational/ClassMetamodel.vio: examples/Class2Relational/ClassMetamodel.v core/utils/tTop.vio core/Metamodel.vio core/Model.vio core/Object.vio
+examples/Class2Relational/ClassMetamodelPattern.vo examples/Class2Relational/ClassMetamodelPattern.glob examples/Class2Relational/ClassMetamodelPattern.v.beautified: examples/Class2Relational/ClassMetamodelPattern.v examples/Class2Relational/ClassMetamodel.vo
+examples/Class2Relational/ClassMetamodelPattern.vio: examples/Class2Relational/ClassMetamodelPattern.v examples/Class2Relational/ClassMetamodel.vio
+examples/Class2Relational/RelationalMetamodel.vo examples/Class2Relational/RelationalMetamodel.glob examples/Class2Relational/RelationalMetamodel.v.beautified: examples/Class2Relational/RelationalMetamodel.v core/utils/tTop.vo core/Metamodel.vo core/Model.vo core/Object.vo
+examples/Class2Relational/RelationalMetamodel.vio: examples/Class2Relational/RelationalMetamodel.v core/utils/tTop.vio core/Metamodel.vio core/Model.vio core/Object.vio
+examples/Class2Relational/RelationalMetamodelPattern.vo examples/Class2Relational/RelationalMetamodelPattern.glob examples/Class2Relational/RelationalMetamodelPattern.v.beautified: examples/Class2Relational/RelationalMetamodelPattern.v examples/Class2Relational/RelationalMetamodel.vo
+examples/Class2Relational/RelationalMetamodelPattern.vio: examples/Class2Relational/RelationalMetamodelPattern.v examples/Class2Relational/RelationalMetamodel.vio
+examples/Class2Relational/Class2Relational.vo examples/Class2Relational/Class2Relational.glob examples/Class2Relational/Class2Relational.v.beautified: examples/Class2Relational/Class2Relational.v core/utils/tTop.vo core/Notations.vo core/CoqTL.vo examples/Class2Relational/ClassMetamodel.vo examples/Class2Relational/RelationalMetamodel.vo examples/Class2Relational/ClassMetamodelPattern.vo
+examples/Class2Relational/Class2Relational.vio: examples/Class2Relational/Class2Relational.v core/utils/tTop.vio core/Notations.vio core/CoqTL.vio examples/Class2Relational/ClassMetamodel.vio examples/Class2Relational/RelationalMetamodel.vio examples/Class2Relational/ClassMetamodelPattern.vio
 examples/Class2Relational/PersonModel.vo examples/Class2Relational/PersonModel.glob examples/Class2Relational/PersonModel.v.beautified: examples/Class2Relational/PersonModel.v core/Model.vo examples/Class2Relational/ClassMetamodel.vo
 examples/Class2Relational/PersonModel.vio: examples/Class2Relational/PersonModel.v core/Model.vio examples/Class2Relational/ClassMetamodel.vio
-examples/Class2RelationalMV/ClassMetamodel.vo examples/Class2RelationalMV/ClassMetamodel.glob examples/Class2RelationalMV/ClassMetamodel.v.beautified: examples/Class2RelationalMV/ClassMetamodel.v core/utils/tTop.vo core/Metamodel.vo core/Model.vo
-examples/Class2RelationalMV/ClassMetamodel.vio: examples/Class2RelationalMV/ClassMetamodel.v core/utils/tTop.vio core/Metamodel.vio core/Model.vio
-examples/Class2RelationalMV/RelationalMetamodel.vo examples/Class2RelationalMV/RelationalMetamodel.glob examples/Class2RelationalMV/RelationalMetamodel.v.beautified: examples/Class2RelationalMV/RelationalMetamodel.v core/utils/tTop.vo core/Metamodel.vo core/Model.vo
-examples/Class2RelationalMV/RelationalMetamodel.vio: examples/Class2RelationalMV/RelationalMetamodel.v core/utils/tTop.vio core/Metamodel.vio core/Model.vio
-examples/Class2RelationalMV/Class2Relational.vo examples/Class2RelationalMV/Class2Relational.glob examples/Class2RelationalMV/Class2Relational.v.beautified: examples/Class2RelationalMV/Class2Relational.v core/utils/tTop.vo core/Notations.vo core/CoqTL.vo examples/Class2RelationalMV/ClassMetamodel.vo examples/Class2RelationalMV/RelationalMetamodel.vo
-examples/Class2RelationalMV/Class2Relational.vio: examples/Class2RelationalMV/Class2Relational.v core/utils/tTop.vio core/Notations.vio core/CoqTL.vio examples/Class2RelationalMV/ClassMetamodel.vio examples/Class2RelationalMV/RelationalMetamodel.vio
+examples/Class2RelationalMV/ClassMetamodel.vo examples/Class2RelationalMV/ClassMetamodel.glob examples/Class2RelationalMV/ClassMetamodel.v.beautified: examples/Class2RelationalMV/ClassMetamodel.v core/utils/tTop.vo core/Metamodel.vo core/Model.vo core/Object.vo
+examples/Class2RelationalMV/ClassMetamodel.vio: examples/Class2RelationalMV/ClassMetamodel.v core/utils/tTop.vio core/Metamodel.vio core/Model.vio core/Object.vio
+examples/Class2RelationalMV/ClassMetamodelPattern.vo examples/Class2RelationalMV/ClassMetamodelPattern.glob examples/Class2RelationalMV/ClassMetamodelPattern.v.beautified: examples/Class2RelationalMV/ClassMetamodelPattern.v examples/Class2RelationalMV/ClassMetamodel.vo
+examples/Class2RelationalMV/ClassMetamodelPattern.vio: examples/Class2RelationalMV/ClassMetamodelPattern.v examples/Class2RelationalMV/ClassMetamodel.vio
+examples/Class2RelationalMV/RelationalMetamodel.vo examples/Class2RelationalMV/RelationalMetamodel.glob examples/Class2RelationalMV/RelationalMetamodel.v.beautified: examples/Class2RelationalMV/RelationalMetamodel.v core/utils/tTop.vo core/Metamodel.vo core/Model.vo core/Object.vo
+examples/Class2RelationalMV/RelationalMetamodel.vio: examples/Class2RelationalMV/RelationalMetamodel.v core/utils/tTop.vio core/Metamodel.vio core/Model.vio core/Object.vio
+examples/Class2RelationalMV/RelationalMetamodelPattern.vo examples/Class2RelationalMV/RelationalMetamodelPattern.glob examples/Class2RelationalMV/RelationalMetamodelPattern.v.beautified: examples/Class2RelationalMV/RelationalMetamodelPattern.v examples/Class2RelationalMV/RelationalMetamodel.vo
+examples/Class2RelationalMV/RelationalMetamodelPattern.vio: examples/Class2RelationalMV/RelationalMetamodelPattern.v examples/Class2RelationalMV/RelationalMetamodel.vio
+examples/Class2RelationalMV/Class2Relational.vo examples/Class2RelationalMV/Class2Relational.glob examples/Class2RelationalMV/Class2Relational.v.beautified: examples/Class2RelationalMV/Class2Relational.v core/utils/tTop.vo core/Notations.vo core/CoqTL.vo examples/Class2RelationalMV/ClassMetamodel.vo examples/Class2RelationalMV/RelationalMetamodel.vo examples/Class2RelationalMV/ClassMetamodelPattern.vo
+examples/Class2RelationalMV/Class2Relational.vio: examples/Class2RelationalMV/Class2Relational.v core/utils/tTop.vio core/Notations.vio core/CoqTL.vio examples/Class2RelationalMV/ClassMetamodel.vio examples/Class2RelationalMV/RelationalMetamodel.vio examples/Class2RelationalMV/ClassMetamodelPattern.vio
 examples/Class2RelationalMV/PersonModel.vo examples/Class2RelationalMV/PersonModel.glob examples/Class2RelationalMV/PersonModel.v.beautified: examples/Class2RelationalMV/PersonModel.v core/Model.vo examples/Class2RelationalMV/ClassMetamodel.vo
 examples/Class2RelationalMV/PersonModel.vio: examples/Class2RelationalMV/PersonModel.v core/Model.vio examples/Class2RelationalMV/ClassMetamodel.vio
+examples/ClassGraph2Tree/ClassMetamodel.vo examples/ClassGraph2Tree/ClassMetamodel.glob examples/ClassGraph2Tree/ClassMetamodel.v.beautified: examples/ClassGraph2Tree/ClassMetamodel.v core/utils/tTop.vo core/Metamodel.vo core/Model.vo core/Object.vo
+examples/ClassGraph2Tree/ClassMetamodel.vio: examples/ClassGraph2Tree/ClassMetamodel.v core/utils/tTop.vio core/Metamodel.vio core/Model.vio core/Object.vio
+examples/ClassGraph2Tree/ClassMetamodelPattern.vo examples/ClassGraph2Tree/ClassMetamodelPattern.glob examples/ClassGraph2Tree/ClassMetamodelPattern.v.beautified: examples/ClassGraph2Tree/ClassMetamodelPattern.v examples/ClassGraph2Tree/ClassMetamodel.vo
+examples/ClassGraph2Tree/ClassMetamodelPattern.vio: examples/ClassGraph2Tree/ClassMetamodelPattern.v examples/ClassGraph2Tree/ClassMetamodel.vio
+examples/ClassGraph2Tree/ClassGraph2Tree.vo examples/ClassGraph2Tree/ClassGraph2Tree.glob examples/ClassGraph2Tree/ClassGraph2Tree.v.beautified: examples/ClassGraph2Tree/ClassGraph2Tree.v core/utils/tTop.vo core/Notations.vo core/Model.vo core/CoqTL.vo examples/ClassGraph2Tree/ClassMetamodel.vo examples/ClassGraph2Tree/ClassMetamodelPattern.vo
+examples/ClassGraph2Tree/ClassGraph2Tree.vio: examples/ClassGraph2Tree/ClassGraph2Tree.v core/utils/tTop.vio core/Notations.vio core/Model.vio core/CoqTL.vio examples/ClassGraph2Tree/ClassMetamodel.vio examples/ClassGraph2Tree/ClassMetamodelPattern.vio
+examples/ClassGraph2Tree/PersonModel.vo examples/ClassGraph2Tree/PersonModel.glob examples/ClassGraph2Tree/PersonModel.v.beautified: examples/ClassGraph2Tree/PersonModel.v core/Model.vo examples/ClassGraph2Tree/ClassMetamodel.vo
+examples/ClassGraph2Tree/PersonModel.vio: examples/ClassGraph2Tree/PersonModel.v core/Model.vio examples/ClassGraph2Tree/ClassMetamodel.vio
